Un "auto" [dll_valid_and_unchanged_through_pop]

ind/DoublyLinkedListIface.fst
@@ -166,14 +166,12 @@ let _auto_dll_valid_and_unchanged_through_push h0 h1 d =
   _lemma_nodelist_conn_in_unmodified_mem h0 h1 B.loc_none (as_list h1 d)
 
 (** If a frame is popped, then a dll remains valid and unchanged. *)
-val _auto_dll_valid_and_unchanged_through_pop (h0 h1:HS.mem) (d:dll 'a) :
+val _lemma_dll_valid_and_unchanged_through_pop (h0 h1:HS.mem) (d:dll 'a) :
   Lemma
     (requires (dll_valid h0 d /\ HS.popped h0 h1 /\
               B.loc_disjoint (fp_dll h0 d) (B.loc_all_regions_from false (HS.get_tip h0))))
     (ensures (dll_valid h1 d /\ d@h0 == d@h1))
-    [SMTPat (dll_valid h0 d);
-     SMTPat (HS.popped h0 h1)]
-let _auto_dll_valid_and_unchanged_through_pop h0 h1 d =
+let _lemma_dll_valid_and_unchanged_through_pop h0 h1 d =
   B.popped_modifies h0 h1;
   assert (B.loc_all_regions_from false (HS.get_tip h0) `B.loc_includes`
             B.loc_region_only false (HS.get_tip h0)); // OBSERVE
